<?xml version="1.0" encoding="UTF-8" ?>
<section xml:id="sec_det_prop_exam">
  <title>Examples</title>
  <p>
    What follows are worked examples that use the concepts from this section.
  </p>

  <example>
    
        <task>
          <introduction>
            <p>
              If <m>A</m>, <m>B</m> are <m>n\times n</m> matrices with
              <m>\det(A)=3</m> and <m>\det(B)=2</m>,
              evaluate the following determinant values.
              Briefly justify.
            </p>
          </introduction>
              <task>
                <statement>
                  <p>
                    <m>\det(A^{-1})</m>
                  </p>
                </statement>
                <solution>
                  <p>
                    Assume that <m>\det(A)=3</m> and <m>\det(B)=2</m>.
                  </p>
                  <p>
                    Since <m>\det(A) \neq 0</m>, we know that <m>A</m> is invertible.
                    Since <m>1 = \det(I_n) = \det(AA^{-1}) = \det(A) \det(A^{-1})</m>,
                    it follows that <m>\det(A^{-1}) = \frac{1}{\det(A)} = \frac{1}{3}</m>.
                  </p>
                </solution>
              </task>
              <task>
                <statement>
                  <p>
                    <m>\det(ABA^{\mathsf{T}})</m>
                  </p>
                </statement>
                <solution>
                  <p>
                    Assume that <m>\det(A)=3</m> and <m>\det(B)=2</m>.
                  </p>
                  <p>
                    We know that <m>\det(A^{\tr}) = \det(A)</m>, so
                    <md>
                      <mrow>\det(ABA^\tr) \amp = \det(A) \det(B) \det(A^{\tr})</mrow>
                      <mrow>\amp = \det(A) \det(B) \det(A)</mrow>
                      <mrow>\amp = (3)(2)(3)</mrow>
                      <mrow>\amp = 18</mrow>
                    </md>.
                  </p>
                </solution>
              </task>
              <task>
                <statement>
                  <p>
                    <m>\det(A^3(BA)^{-1}(AB)^2)</m>
                  </p>
                </statement>
                <solution>
                  <p>
                    Assume that <m>\det(A)=3</m> and <m>\det(B)=2</m>.
                  </p>
                  <p>
                    Using properties of determinants gives us
                    <md>
                      <mrow>\det(A^3(BA)^{-1}(AB)^2) \amp = \det(A^3)\det((BA)^{-1}) \det((AB)^2)</mrow>
                      <mrow>\amp = (\det(A))^3 \left(\frac{1}{\det(AB)}\right) (\det(AB))^2</mrow>
                      <mrow>\amp = 27 \left(\frac{1}{\det(A) \det(B)} \right) (\det(A)\det(B))^2</mrow>
                      <mrow>\amp = \frac{(27)(6^2)}{6}</mrow>
                      <mrow>\amp = 162</mrow>
                    </md>.
                  </p>
                </solution>
              </task>
        </task>

        <task>
          <introduction>
            <p>
              If the determinant of <m>\left[ \begin{array}{ccc} a\amp b\amp c\\d\amp e\amp f\\g\amp h\amp i \end{array} \right]</m> is <m>m</m>,
              find the determinant of each of the following matrices.
            </p>
          </introduction>
              <task>
                <statement>
                  <p>
                    <m>\left[ \begin{array}{ccc} a\amp b\amp c\\2d\amp 2e\amp 2f\\g\amp h\amp i \end{array} \right]</m>
                  </p>
                </statement>
                <solution>
                  <p>
                    Assume that <m>\det\left(\left[ \begin{array}{ccc} a\amp b\amp c\\d\amp e\amp f\\g\amp h\amp i \end{array}  \right] \right) = m</m>.
                  </p>
                  <p>
                    Multiplying a row by a scalar multiples the determinant by that scalar, so
                    <me>
                      \det\left( \left[ \begin{array}{ccc} a\amp b\amp c\\2d\amp 2e\amp 2f\\g\amp h\amp i \end{array}  \right] \right) = 2m
                    </me>.
                  </p>
                </solution>
              </task>
              <task>
                <statement>
                  <p>
                    <m>\left[ \begin{array}{ccc} d\amp e\amp f\\g\amp h\amp i\\a\amp b\amp c \end{array} \right]</m>
                  </p>
                </statement>
                <solution>
                  <p>
                    Assume that <m>\det\left(\left[ \begin{array}{ccc} a\amp b\amp c\\d\amp e\amp f\\g\amp h\amp i \end{array}  \right] \right) = m</m>.
                  </p>
                  <p>
                    Interchanging two rows multiples the determinant by <m>-1</m>.
                    It takes two row swaps in the original matrix to obtain this one, so
                    <me>
                      \det\left( \left[ \begin{array}{ccc} d\amp e\amp f\\g\amp h\amp i\\a\amp b\amp c \end{array}  \right] \right) = (-1)^2m = m
                    </me>.
                  </p>
                </solution>
              </task>
              <task>
                <statement>
                  <p>
                    <m>\left[ \begin{array}{ccc} a\amp b\amp c\\g-2d\amp h-2e\amp i-2f\\a+d\amp b+e\amp c+f \end{array} \right]</m>
                  </p>
                </statement>
                <solution>
                  <p>
                    Assume that <m>\det\left(\left[ \begin{array}{ccc} a\amp b\amp c\\d\amp e\amp f\\g\amp h\amp i \end{array}  \right] \right) = m</m>.
                  </p>
                  <p>
                    Adding a multiple of a row to another does not change the determinant of the matrix.
                    Since there is a row swap needed to get this matrix from the original we have
                    <me>
                      \det\left(\left[ \begin{array}{ccc} a\amp b\amp c\\g-2d\amp h-2e\amp i-2f\\a+d\amp b+e\amp c+f \end{array}  \right]\right) = -m
                    </me>.
                  </p>
                </solution>
              </task>
        
        </task>
      
  </example>

  <example>
    <introduction>
      <p>
        Let <m>A = \left[ \begin{array}{ccr} 2\amp 8\amp 0\\2\amp 2\amp -3\\1\amp 2\amp 7 \end{array} \right]</m>.
      </p>
    </introduction>
        <task>
          <statement>
            <p>
              Find an LU factorization for <m>A</m>.
            </p>
          </statement>
          <solution>
            <p>
              We row reduce <m>A</m> to an upper triangular matrix by applying elementary matrices.
              First notice that if <m>E_1 = \left[ \begin{array}{rcc} 1\amp 0\amp 0 \\-1\amp 1\amp 0 \\ 0\amp 0\amp 1 \end{array}  \right]</m>, then
              <me>
                E_1 A = \left[ \begin{array}{crr} 2\amp 8\amp 0 \\ 0\amp -6\amp -3 \\ 1\amp 2\amp 7 \end{array}  \right]
              </me>.
              Letting <m>E_2 =  \left[ \begin{array}{rcc} 1\amp 0\amp 0 \\0\amp 1\amp 0 \\ -\frac{1}{2}\amp 0\amp 1 \end{array}  \right]</m> gives us
              <me>
                E_2E_1A = \left[ \begin{array}{crr} 2\amp 8\amp 0 \\ 0\amp -6\amp -3 \\ 0\amp -2\amp 7 \end{array}  \right]
              </me>.
              Finally, when <m>E_3 = \left[ \begin{array}{crc} 1\amp 0\amp 0 \\0\amp 1\amp 0 \\ 0\amp -\frac{1}{3}\amp 1 \end{array}  \right]</m> we have
              <me>
                U=E_3E_2E_1A = \left[ \begin{array}{crr} 2\amp 8\amp 0 \\ 0\amp -6\amp -3 \\ 0\amp 0\amp 8 \end{array}  \right]
              </me>.
              This gives us <m>E_3E_2E_1A = U</m>, so we can take
              <me>
                L = E_1^{-1}E_2^{-1}E_3^{-1} =  \left[ \begin{array}{ccc} 1\amp 0\amp 0 \\1\amp 1\amp 0 \\ \frac{1}{2}\amp \frac{1}{3}\amp 1 \end{array}  \right]
              </me>.
            </p>
          </solution>
        </task>
        <task>
          <statement>
            <p>
              Use the LU factorization with forward substitution and back substitution to solve the system <m>A \vx = [18 \ 3 \ 12]^{\tr}</m>.
            </p>
          </statement>
          <solution>
            <p>
              To solve the system <m>A \vx = \vb</m>,
              where <m>\vb = [18 \ 3 \ 12]^{\tr}</m>,
              we use the LU factorization of <m>A</m> and solve <m>LU \vx = \vb</m>.
              Let <m>\vx = [x_1 \ x_2 \ x_3]^{\tr}</m> and let <m>\vz = [z_1 \ z_2 \ z_3]^{\tr}</m> with
              <m>U \vx = \vz</m> so that <m>L \vz = L(U\vx) = A\vx = \vb</m>.
              First we solve <m>L \vz = [18 \ 3 \ 12]^{\tr}</m> to find <m>\vz</m> using forward substitution.
              The first row of <m>L</m> shows that
              <m>z_1 = 18</m> and the second row that <m>z_1 + z_2 = 3</m>.
              So <m>z_2 = -15</m>.
              The third row of <m>L</m> gives us <m>\frac{1}{2}z_1 + \frac{1}{3}z_2 + z_3 = 12</m>,
              so <m>z_3 = 12 - 9 + 5 = 8</m>.
              Now to find <m>\vx</m> we solve
              <m>U \vx = \vz</m> using back substitution.
              The third row of <m>U</m> tells us that
              <m>8x_3 = 8</m> or that <m>x_3 = 1</m>.
              The second row of <m>U</m> shows that <m>-6x_2-3x_3 = -15</m> or <m>x_2 =2</m>.
              Finally, the first row of <m>U</m> gives us <m>2x_1+8x_2 = 18</m>,
              or <m>x_1 = 1</m>.
              So the solution to <m>A \vx = \vb</m> is <m>\vx = [1 \ 2 \ 1]^{\tr}</m>.
            </p>
          </solution>
        </task>
      
  </example>
</section>