<?xml version="1.0" encoding="UTF-8" ?>
<section xml:id="sec_vec_space_exam">
  <title>Examples</title>
  <p>
    What follows are worked examples that use the concepts from this section.
  </p>
  <example>
    <statement>
      <p>
        Determine if each of the following sets is a vector space.
        <ul>
          <li>
            <p>
              <m>V = \{(x,y,z) : x,y,z \in \R\}</m> with addition and multiplication by scalars defined by
              <me>
                (a,b,c) \oplus (x,y,z) = (a+x, c+z, b+y) \ \text{ and }  \ k(x,y,z) = (kx,kz,ky)
              </me>,
              where <m>(a,b,c)</m> and <m>(x,y,z)</m> are in <m>V</m> and <m>k \in \R</m>
            </p>
          </li>
          <li>
            <p>
              <m>V = \{x \in \R : x > 0\}</m> with addition <m>\oplus</m> and multiplication by scalars defined by
              <me>
                x \oplus y = xy  \ \text{ and }  \ kx = x^k
              </me>,
              where <m>x</m> and <m>y</m> are in <m>V</m>, <m>k \in \R</m>,
              and <m>xy</m> is the standard product of <m>x</m> and <m>y</m>
            </p>
          </li>
          <li>
            <p>
              The set <m>W</m> of all <m>2 \times 2</m> matrices of the form
              <m>\left[ \begin{array}{cc} a\amp 0\\b\amp 0 \end{array} \right]</m> where <m>a</m> and <m>b</m> are real numbers using the standard addition and multiplication by scalars on matrices.
            </p>
          </li>
          <li>
            <p>
              The set <m>W</m> of all functions <m>f</m> from <m>\R</m> to <m>\R</m> such that
              <m>f(0) \geq 0</m> using the standard addition and multiplication by scalars on functions.
            </p>
          </li>
        </ul>
      </p>
      <p>
        <em>Example Solution. </em>
        <ul>
          <li>
            <p>
              We consider the vector space properties in <xref ref="def_vector_space">Definition</xref>.
              Let <m>(a,b,c)</m>, <m>(u,v,w)</m>,
              and <m>(x,y,z)</m> be in <m>V</m> and let <m>k,m  \in \R</m>.
              By the definition of addition and multiplication by scalars,
              both <m>(a,b,c) + (x,y,z)</m> and <m>k (x,y,z)</m> are in <m>V</m>.
              Note also that
              <md>
                <mrow>(a,b,c) \oplus (x,y,z) \amp = (a+x, c+z, b+y)</mrow>
                <mrow>\amp = (x+a, z+c, y+b)</mrow>
                <mrow>\amp = (x,y,z) \oplus (a,b,c)</mrow>
              </md>,
              and so addition is commutative in <m>V</m>.
              Since
              <me>
                ((1,1,0)\oplus(0,1,1)) \oplus (0,0,1) = (1,1,2) \oplus (0,0,1) = (1,3,1)
              </me>
              and
              <me>
                (1,1,0)\oplus ((0,1,1) \oplus (0,0,1)) = (1,1,0) \oplus (0,2,1) = (1,1,3)
              </me>,
              we see that addition is not associative and conclude that <m>V</m> is not a vector space.
              At this point we can stop since we have shown that <m>V</m> is not a vector space.
            </p>
          </li>
          <li>
            <p>
              We consider the vector space properties in <xref ref="def_vector_space">Definition</xref>.
              Let <m>x</m>, <m>y</m>,
              and <m>z</m> be in <m>V</m> and let <m>k,m  \in \R</m>.
              Since <m>x</m> and <m>y</m> are both positive real numbers,
              we know that <m>xy</m> is a positive real number.
              Thus, <m>x \oplus y \in V</m> and <m>V</m> is closed under its addition.
              Also, <m>x^k</m> is a positive real number,
              so <m>x^k \in V</m> as well.
              Now
              <me>
                x \oplus y = xy = yx = y \oplus x
              </me>
              and addition is commutative in <m>V</m>.
              Also,
              <me>
                (x \oplus y) \oplus z = (xy) \oplus z = (xy)z = x(yz) = x \oplus (yz) = x \oplus (y \oplus z)
              </me>
              and addition is associative in <m>V</m>.
              Since
              <me>
                1 \oplus x = 1x = x
              </me>,
              <m>V</m> contains an additive identity, which is <m>1</m>.
              The fact that <m>x</m> is a positive real number implies that
              <m>\frac{1}{x}</m> is a positive real number.
              Thus, <m>\frac{1}{x} \in V</m> and
              <me>
                x \oplus \frac{1}{x} = x\left(\frac{1}{x}\right) = 1
              </me>
              and <m>V</m> contains an additive inverse for each of its elements.
              We have that
              <md>
                <mrow>(k+m)x \amp = x^{k+m} = x^kx^m = x^k \oplus x^m = k(x) \oplus m(x),</mrow>
                <mrow>k(x \oplus +y) \amp = k(xy) = x^ky^k = x^k \oplus y^k = k(x) \oplus k(y),</mrow>
                <mrow>(km)x \amp = x^{km} = \left(x^m\right)^k = (m(x))^k = k(m(x))</mrow>
                <mrow>1x \amp = x^1 = x</mrow>
              </md>.
              So <m>V</m> satisfies all of the properties of a vector space.
            </p>
          </li>
          <li>
            <p>
              Recall that <m>\M_{2 \times 2}</m> is a vector space using the standard addition and multiplication by scalars on matrices.
              Any matrix of the form <m>\left[ \begin{array}{cc} a\amp 0\\b\amp 0 \end{array}  \right]</m>  can be written as
              <me>
                \left[ \begin{array}{cc} a\amp 0\\b\amp 0 \end{array}  \right] = a\left[ \begin{array}{cc} 1\amp 0\\0\amp 0 \end{array}  \right]  + b \left[ \begin{array}{cc} 0\amp 0\\1\amp 0 \end{array}  \right]
              </me>.
              So <m>W = \Span\left\{\left[ \begin{array}{cc} 1\amp 0\\0\amp 0 \end{array}  \right],  \left[ \begin{array}{cc} 0\amp 0\\1\amp 0 \end{array}  \right]\right\}</m> and <m>W</m> is a subspace of <m>\M_{2 \times 2}</m>.
              Thus, <m>W</m> is a vector space.
            </p>
          </li>
          <li>
            <p>
              We will show that <m>W</m> is not a vector space.
              Let <m>f: \R \to \R</m> be defined by <m>f(x) = 1</m>.
              Then <m>f(0) \geq 0</m> and <m>f \in W</m>.
              However, if <m>h = (-1)f</m>,
              then <m>h(0) = (-1)f(0) = -1</m> and <m>h \notin W</m>.
              It follows that <m>W</m> is not closed under multiplication by scalars and <m>W</m> is not a vector space.
            </p>
          </li>
        </ul>
      </p>
    </statement>
  </example>
  <example>
    <statement>
      <p>
        Let <m>V</m> be a vector space and <m>\vu</m> and <m>\vv</m> vectors in <m>V</m>.
        Also, let <m>a</m> and <m>b</m> be scalars.
        You may use the result of <xref ref="ex_5_a_scalar_times_0"></xref>
        that <m>c \vzero = \vzero</m> for any scalar <m>c</m> in any vector space.
        <ul>
          <li>
            <p>
              If <m>a \vv = b \vv</m> and <m>\vv \neq \vzero</m>, must <m>a = b</m>?
              Use the properties of a vector space or provide a counterexample to justify your answer.
            </p>
          </li>
          <li>
            <p>
              If <m>a \vu = a \vv</m> and
              <m>a \neq 0</m>, must <m>\vu = \vv</m>?
              Use the properties of a vector space or provide a counterexample to justify your answer.
            </p>
          </li>
          <li>
            <p>
              If <m>a\vu = b\vv</m>, must <m>a = b</m> and <m>\vu = \vv</m>?
              Use the properties of a vector space or provide a counterexample to justify your answer.
            </p>
          </li>
        </ul>
      </p>
      <p>
        <em>Example Solution. </em>
        <ul>
          <li>
            <p>
              We will show that this statement is true.
              Suppose <m>a \vv = b \vv</m> and <m>\vv \neq \vzero</m>.
              Then <m>\vzero = a \vv - b \vv = (a-b)\vv</m>.
              If <m>a = b</m>, then we are done.
              So suppose <m>a \neq b</m>.
              Then <m>a-b \neq 0</m> and <m>\frac{1}{a-b}</m> is a real number.
              Then
              <md>
                <mrow>\frac{1}{a-b} \vzero \amp = \frac{1}{a-b}((a-b)\vv)</mrow>
                <mrow>\vzero \amp = \left(\frac{1}{a-b}(a-b)\right) \vv</mrow>
                <mrow>\vzero \amp = \vv</mrow>
              </md>.
              But we assumed that <m>\vv \neq \vzero</m>,
              so we can conclude that <m>a = b</m> as desired.
            </p>
          </li>
          <li>
            <p>
              We will show that this statement is true.
              Suppose <m>a \vu = a \vv</m> and <m>a \neq 0</m>.
              Then <m>\vzero = a \vu - a \vv = a(\vu - \vv)</m>.
              Since <m>a \neq 0</m>, we know that <m>\frac{1}{a}</m> is a real number.
              Thus,
              <md>
                <mrow>\frac{1}{a} \vzero \amp = \frac{1}{a} \left(a (\vu - \vv)\right)</mrow>
                <mrow>\vzero \amp = \left( \frac{1}{a}a\right) (\vu - \vv)</mrow>
                <mrow>\vzero \amp = \vu - \vv</mrow>
                <mrow>\vu \amp = \vv</mrow>
              </md>.
            </p>
          </li>
          <li>
            <p>
              We will demonstrate that this statement is false with a counterexample.
              Let <m>a = 1</m>, <m>b = 2</m>,
              <m>\vu = [2 \ 0]^{\tr}</m> and <m>\vv = [1 \ 0]^{\tr}</m> in <m>\R^2</m>.
              Then
              <me>
                a \vu = 1[2 \ 0]^{\tr} = [2 \ 0]^{\tr} = 2[1 \ 0]^{\tr} = b \vv
              </me>,
              but <m>a \neq b</m> and <m>\vu \neq \vv</m>.
            </p>
          </li>
        </ul>
      </p>
    </statement>
  </example>
</section>