<?xml version="1.0" encoding="UTF-8" ?>
<section xml:id="sec_proj_sum_powers">
  <title>Project: Finding Formulas for Sums of Powers</title>
  <p>
    One way to derive formulas for sums of powers of whole numbers is to use different bases and coordinate vectors.
    One basis that will be useful is a basis of polynomials created by the binomial coefficients.
    Recall that the binomial coefficient <m>\binom{n}{k}</m> is equal to
    <me>
      \binom{n}{k} = \frac{n!}{k!(n-k)!}
    </me>,
    with <m>\binom{n}{k} = 0</m> if <m>n \lt  k</m>.
  </p>
  <p>
    The binomial coefficient can be rewritten in a way to make it applicable to polynomials as
    <me>
      \binom{n}{k} = \frac{n(n-1)(n-2) \cdots (n-k+1)}{k!} = \Pi_{i=1}^k \frac{1}{i}(n-i+1)
    </me>.
  </p>
  <p>
    With this representation of <m>\binom{n}{k}</m>,
    we can define a new polynomial in <m>t</m> of degree <m>k</m> as
    <me>
      p_{k}(t) = \frac{1}{k!}(t)(t-1)(t-2) \cdots (t-k+1)
    </me>
    with <m>p_0(t) = 1</m>.
    For example,
    <md>
      <mrow>p_1(t) \amp = \frac{1}{1!}t = t</mrow>
      <mrow>p_2(t) \amp = \frac{1}{2}(t)(t-1) = \frac{1}{2}\left(t^2-t\right)</mrow>
      <mrow>p_3(t) \amp = \frac{1}{6}(t)(t-1)(t-2) = \frac{1}{6}\left(t^3-3t^2+2t\right)</mrow>
    </md>.
  </p>
  <p>
    These
    <q>generalized binomial coefficients</q>
    appear in Newton's generalized binomial theorem.
  </p>
  <p>
    Two facts will make these polynomials useful for our sums.
  </p>
  <activity xml:id="act_hockey_stick">
    <p>
      Our polynomials <m>p_k(t)</m> are defined in terms of binomial coefficients.
      A useful identity will relate sums of binomial coefficients to other binomial coefficients.
      This identity, called the <em>hockey-stick identity</em>
      after the way it can be visualized on Pascal's triangle,
      is as follows:
      <me>
        \sum_{k=0}^{n-1} \binom{k}{r} = \binom{n}{r+1}
      </me>
      for positive integers <m>r</m>.
      Use the definition of the binomial coefficients and some algebra to verify the hockey-stick identity.
    </p>
  </activity>
  <p>
    The second useful fact about our polynomials <m>p_k(t)</m> is that they form a basis for <m>\pol_n</m>.
  </p>
  <activity xml:id="act_binomial_basis">
    <p>
      <nbsp/>
      <ul>
        <li>
          <p>
            Let <m>k</m> be a positive integer.
            Explain why <m>p_k(0) = p_k(1) = p_k(2) = \cdots = p_k(k-1) = 0</m> and <m>p_k(k) = 1</m>.
          </p>
        </li>
        <li>
          <p>
            Let <m>\CP_n = \{p_0(t), p_1(t),
            p_2(t), \ldots, p_n(t)\}</m>.
            Show that <m>\CP_n</m> is a basis for <m>\pol_n</m>. (Hint: Let <m>c_1</m>,
            <m>c_2</m>,
            <m>\ldots</m>, <m>c_n</m> be scalars and consider the equation
            <me>
              c_0p_0(t) + c_1p_1(t) + c_2 p_2(t) + \cdots + c_np_n(t) = 0
            </me>.
            Evaluate this equation at <m>t=0</m>, <m>t=1</m>,
            <m>\ldots</m>, <m>t=n</m> and use the result of part (a).)
          </p>
        </li>
      </ul>
    </p>
  </activity>
  <p>
    Now we have the tools we need to derive our formulas.
    To simplify computations,
    we will change coordinates to the standard basis <m>\CS_n = \{1, t, t^2, \ldots,
    t^n\}</m> for <m>\pol_n</m>.
  </p>
  <p>
    We will illustrate the process of deriving formulas for our sums with the sum <m>\sum_{t=0}^{n-1} t</m>.
    We want to write <m>t</m> as a linear combination of the vectors in <m>\CP_1</m> so that we can utilize the hockey-stick identity.
    In this case, by definition we have <m>t = p_1(t)</m>.
    It follows by the hockey-stick identity and the fact that <m>p_1(t) = \binom{t}{1}</m> that
    <md>
      <mrow>\sum_{t=0}^{n-1} t \amp = \sum_{t=0}^{n-1}  p_1(t)</mrow>
      <mrow>\amp = \sum_{t=0}^{n-1}  \binom{t}{1}</mrow>
      <mrow>\amp = \binom{n}{2}</mrow>
      <mrow>\amp = \frac{1}{2}\left(n^2-n\right)</mrow>
    </md>.
  </p>
  <p>
    This is exactly the formula we saw at the beginning of this section.
    The cases for sums of higher powers work the same way,
    but we will need to do a little more work to write <m>t^n</m> in terms of the basis vectors in <m>\CP_n</m>.
  </p>
  <activity xml:id="act_sum_2">
    <p>
      Consider the sum <m>\sum_{t=0}^{n-1} t^2</m>.
      We want to write <m>t^2</m> as a linear combination of <m>p_0(t)</m>,
      <m>p_1(t)</m> and <m>p_2(t)</m>.
      To do so, we will use the coordinate vectors with respect to <m>\CS_2</m> and do our work in <m>\R^3</m>.
      <ul>
        <li>
          <p>
            Find <m>[p_0(t)]_{\CS_2}</m>,
            <m>[p_1(t)]_{\CS_2}</m>, <m>[p_2(t)]_{\CS_2}</m>, and <m>[t^2]_{\CS_2}</m>.
          </p>
        </li>
        <li>
          <p>
            Use the coordinate vectors from part (a) to write <m>t^2</m> as a linear combination of the vectors in <m>\CP_2</m>.
          </p>
        </li>
        <li>
          <p>
            Use the result of part (b) and,
            the hockey-stick identity,
            and the fact that <m>p_k(t) = \binom{t}{k}</m> to find a formula for <m>\sum_{t=0}^{n-1} t^2</m>.
          </p>
        </li>
      </ul>
    </p>
  </activity>
  <p>
    Deriving formulas for higher powers involves the same process,
    just with more algebra.
  </p>
  <activity xml:id="act_sums_higher">
    <p>
      Use the process outlined in Project <xref ref="act_sum_2">Activity</xref>
      to derive formulas for the following sums.
      <ul>
        <li>
          <p>
            <m>\sum_{t=0}^{n-1} t^3</m>
          </p>
        </li>
        <li>
          <p>
            <m>\sum_{t=0}^{n-1} t^4</m>
          </p>
        </li>
      </ul>
    </p>
  </activity>
</section>