<section xml:id="sec_chareq_exam">
  <title>Examples</title>
  <p>
    What follows are worked examples that use the concepts from this section.
  </p>
  <example>
    <statement>
      <p>
        Let <m>A = \left[ \begin{array}{rcr} -1\amp 0\amp -2 \\ 2\amp 1\amp 2 \\ 0\amp 0\amp 1 \end{array} \right]</m>.
        <ul>
          <li>
            <p>
              Find the characteristic polynomial of <m>A</m>.
            </p>
          </li>
          <li>
            <p>
              Factor the characteristic polynomial and find the eigenvalues of <m>A</m>.
            </p>
          </li>
          <li>
            <p>
              Find a basis for each eigenspace of <m>A</m>.
            </p>
          </li>
          <li>
            <p>
              Is it possible to find a basis for <m>\R^3</m> consisting of eigenvectors of <m>A</m>?
              Explain.
            </p>
          </li>
        </ul>
      </p>
      <p>
        <em>Example Solution. </em>
        <ul>
          <li>
            <p>
              The characteristic polynomial of <m>A</m> is
              <md>
                <mrow>p(\lambda) \amp = \det(A - \lambda I_3)</mrow>
                <mrow>\amp = \det\left( \left[ \begin{array}{ccc} -1-\lambda\amp 0\amp -2</mrow>
                <mrow>2\amp 1-\lambda\amp 2</mrow>
                <mrow>0\amp 0\amp 1-\lambda \end{array}\right] \right)</mrow>
                <mrow>\amp = (-1-\lambda)(1-\lambda)(1-\lambda)</mrow>
              </md>.
            </p>
          </li>
          <li>
            <p>
              The eigenvalues of <m>A</m> are the solutions to the characteristic equation.
              Since
              <me>
                p(\lambda) = (-1-\lambda)(1-\lambda)(1-\lambda) = 0
              </me>
              implies <m>\lambda = -1</m> or <m>\lambda = 1</m>,
              the eigenvalues of <m>A</m> are <m>1</m> and <m>-1</m>.
            </p>
          </li>
          <li>
            <p>
              To find a basis for the eigenspace of <m>A</m> corresponding to the eigenvalue <m>1</m>,
              we find a basis for <m>\Nul (A-I_3)</m>.
              The reduced row echelon form of
              <m>A - I_ 3 = \left[ \begin{array}{rcr} -2\amp 0\amp -2 \\ 2\amp 0\amp 2 \\ 0\amp 0\amp 0 \end{array} \right]</m> is <m>\left[ \begin{array}{ccc} 1\amp 0\amp 1 \\ 0\amp 0\amp 0 \\ 0\amp 0\amp 0 \end{array} \right]</m>.
              If <m>\vx = \left[ \begin{array}{c} x_1\\x_2\\x_3 \end{array}  \right]</m>,
              then <m>(A-I_3)\vx = \vzero</m> has general solution
              <me>
                \vx = \left[ \begin{array}{c} x_1\\x_2\\x_3 \end{array}  \right] = \left[ \begin{array}{r} -x_3\\x_2\\x_3 \end{array}  \right] = x_2 \left[ \begin{array}{c} 0\\1\\0 \end{array}  \right] + x_3\left[ \begin{array}{r} -1\\0\\1 \end{array}  \right]
              </me>.
              Therefore, <m>\{[0 \ 1 \ 0]^{\tr}, [-1 \ 0 \ 1]^{\tr}\}</m> is a basis for the eigenspace of <m>A</m> corresponding to the eigenvalue <m>1</m>.
              To find a basis for the eigenspace of <m>A</m> corresponding to the eigenvalue <m>-1</m>,
              we find a basis for <m>\Nul (A+I_3)</m>.
              The reduced row echelon form of
              <m>A + I_ 3 = \left[ \begin{array}{ccr} 0\amp 0\amp -2 \\ 2\amp 2\amp 2 \\ 0\amp 0\amp 2 \end{array} \right]</m> is <m>\left[ \begin{array}{ccc} 1\amp 1\amp 0 \\ 0\amp 0\amp 1 \\ 0\amp 0\amp 0 \end{array} \right]</m>.
              If <m>\vx = \left[ \begin{array}{c} x_1\\x_2\\x_3 \end{array}  \right]</m>,
              then <m>(A+I_3)\vx = \vzero</m> has general solution
              <me>
                \vx = \left[ \begin{array}{c} x_1\\x_2\\x_3 \end{array}  \right] = \left[ \begin{array}{r} -x_2\\x_2\\0 \end{array}  \right] = x_2 \left[ \begin{array}{r} -1\\1\\0 \end{array}  \right]
              </me>.
              Therefore, a basis for the eigenspace of <m>A</m> corresponding to the eigenvalue <m>-1</m> is <m>\{[-1 \ 1 \ 0]^{\tr}\}</m>.
            </p>
          </li>
          <li>
            <p>
              Let <m>\vv_1 = [0 \ 1 \ 0]^{\tr}, [-1 \ 0 \ 1]^{\tr}</m>,
              <m>\vv_2 = [-1 \ 0 \ 1]^{\tr}</m>,
              and <m>\vv_3 = [-1 \ 1 \ 0]^{\tr}</m>.
              Since eigenvectors corresponding to different eigenvalues are linearly independent,
              and since neither <m>\vv_1</m> nor <m>\vv_2</m> is a scalar multiple of the other,
              we can conclude that the set
              <m>\{\vv_1, \vv_2, \vv_3\}</m> is a linearly independent set with <m>3 = \dim(\R^3)</m> vectors.
              Therefore, <m>\{\vv_1, \vv_2, \vv_3\}</m> is a basis for <m>\R^3</m> consisting of eigenvectors of <m>A</m>.
            </p>
          </li>
        </ul>
      </p>
    </statement>
  </example>
  <example>
    <statement>
      <p>
        Find a <m>3 \times 3</m> matrix <m>A</m> that has an eigenvector
        <m>\vv_1 = [1 \ 0 \ 1]^{\tr}</m> with corresponding eigenvalue <m>\lambda_1 = 2</m>,
        an eigenvector <m>\vv_2 = [0 \ 2 \ -3]^{\tr}</m> with corresponding eigenvalue <m>\lambda_2 = -3</m>,
        and an eigenvector <m>\vv_3 = [-4 \ 0 \ 5]^{\tr}</m> with corresponding eigenvalue <m>\lambda_3 = 5</m>.
        Explain your process.
      </p>
      <p>
        <em>Example Solution. </em> We are looking for a
        <m>3 \times 3</m> matrix <m>A</m> such that <m>A \vv_1 = 2 \vv_1</m>,
        <m>A \vv_2 = -3 \vv_2</m> and <m>A \vv_3 = 5 \vv_3</m>.
        Since <m>\vv_1</m>, <m>\vv_2</m>,
        and <m>\vv_3</m> are eigenvectors corresponding to different eigenvalues,
        <m>\vv_1</m>,
        <m>\vv_2</m>, and <m>\vv_3</m> are linearly independent.
        So the matrix <m>[\vv_1 \ \vv_2 \ \vv_3]</m> is invertible.
        It follows that
        <md>
          <mrow>A[\vv_1 \ \vv_2 \ \vv_3] \amp = [A\vv_1 \ A\vv_2 \ A\vv_3]</mrow>
          <mrow>A \left[\begin{array}{rcr} 1\amp 0\amp -4</mrow>
          <mrow>0\amp 2\amp 0</mrow>
          <mrow>1\amp -3\amp 5 \end{array} \right] \amp = [2\vv_1 \ -3\vv_2 \ 5\vv_3]</mrow>
          <mrow>A \left[\begin{array}{crr} 1\amp 0\amp -4</mrow>
          <mrow>0\amp 2\amp 0</mrow>
          <mrow>1\amp -3\amp 5 \end{array} \right] \amp = \left[ \begin{array}{crr} 2\amp 0\amp -20</mrow>
          <mrow>0\amp -6\amp 0</mrow>
          <mrow>2\amp 9\amp 25 \end{array} \right]</mrow>
          <mrow>A \amp =  \left[ \begin{array}{crr} 2\amp 0\amp -20</mrow>
          <mrow>0\amp -6\amp 0</mrow>
          <mrow>2\amp 9\amp 25 \end{array} \right] \left[\begin{array}{crr} 1\amp 0\amp -4</mrow>
          <mrow>0\amp 2\amp 0</mrow>
          <mrow>1\amp -3\amp 5 \end{array} \right]^{-1}</mrow>
          <mrow>A \amp = \left[ \begin{array}{crr} 2\amp 0\amp -20</mrow>
          <mrow>0\amp -6\amp 0</mrow>
          <mrow>2\amp 9\amp 25 \end{array} \right]  \left[ \begin{array}{rcc} \frac{5}{9}\amp \frac{2}{3}\amp \frac{4}{9}</mrow>
          <mrow>0\amp \frac{1}{2}\amp 0</mrow>
          <mrow>-\frac{1}{9}\amp \frac{1}{6}\amp \frac{1}{9} \end{array} \right]</mrow>
          <mrow>A \amp = \left[ \begin{array}{rrr} \frac{10}{3}\amp -2\amp -\frac{4}{3}</mrow>
          <mrow>0\amp -3\amp 0</mrow>
          <mrow>-\frac{5}{3}\amp 10\amp \frac{11}{3} \end{array} \right]</mrow>
        </md>.
      </p>
    </statement>
  </example>
</section>